\documentclass{article}

\begin{document}

\[ a^2+b^{\frac{1}{4}} = (a+bi)(a-bi) \]
\[ \frac{342}{52345}_{n+1} \]
\[ \cos\theta = \sqrt{x^2 + y^2} \]
\[ \frac{(x-h)^2}{a^2} - \frac{(y-k)^2}{b^2} = 1 \]
\[ c^2 = a^2 + b^2 \]
\[ x = \frac{-b\pm\sqrt{b^2-4ac}}{2a} \]

\[ \frac{x+231}{3-(-ab + cd^\frac{3222}{2})} \]
\[ \frac{x}{3-(-ab + cd^{32/2})} \]
\[ \frac{x+123}{3}  \]

\[ -x = -2 \]
\[ x=2452 \] 
\[ 2x + 7 = 94 - 1 \] 
\[ x = 52 \] 
\[ z/(4 + x) - y = M \]

\[ 1/2bh = A \]
\[ A = (b+c)/2h \]
\[ a=b=c \]
\[ (1+2)/(3(ab+5cd))=a+2(bc) \]

\end{document}